Fix DCE

DCE.v
@@ -1,6 +1,6 @@
 Require Import CSet Util Fresh Filter MoreExp Take MoreList OUnion.
 Require Import IL Annotation LabelsDefined Sawtooth InRel Liveness UnreachableCode.
-Require Import Sim SimTactics.
+Require Import Sim SimTactics SimI.
 
 Set Implicit Arguments.
 Unset Printing Records.
@@ -20,6 +20,14 @@ Fixpoint countTrue (L:list bool) :=
   | true :: xs => 1 + countTrue xs
   | false :: xs => countTrue xs
   end.
+
+Lemma countTrue_exists (L:list bool) n
+  : get L n true
+    -> countTrue L <> 0.
+Proof.
+  intros. general induction H; simpl; eauto.
+  - cases; eauto.
+Qed.
 
 Lemma countTrue_app (L L':list bool)
   : countTrue (L ++ L') = countTrue L + countTrue L'.
@@ -57,8 +65,10 @@ Fixpoint compile (RZL:list (bool * params)) (s:stmt) (a:ann bool) :=
       stmtExtern x f e (compile RZL s an)
     | stmtFun F t, annF lv ans ant =>
       let LV' := pair ⊜ (getAnn ⊝ ans) (fst ⊝ F) ++ RZL in
-      stmtFun (compileF compile LV' F ans)
-              (compile LV' t ant)
+      match compileF compile LV' F ans with
+      | nil => compile LV' t ant
+      | F' => stmtFun F' (compile LV' t ant)
+      end
     | s, _ => s
   end.
 
@@ -142,8 +152,15 @@ Proof.
   - repeat cases; eauto using isCalled. congruence.
   - simpl in *.
     exploit unreachable_code_trueIsCalled; try eapply IC2; eauto.
-    simpl in *. inv_get.
-    + exploit compileF_get; eauto.
+    simpl in *. inv_get. cases.
+    + exfalso.
+      assert (length (compileF compile (pair ⊜ (getAnn ⊝ als) (fst ⊝ F) ++ pair ⊜ RL ZL) F als)
+              <> 0). {
+        rewrite compileF_length; eauto.
+        eapply countTrue_exists. rewrite H5; eauto using map_get_1.
+      }
+      eapply H1. rewrite <- Heq; eauto.
+    + rewrite Heq; clear Heq. exploit compileF_get; eauto.
       econstructor; eauto.
       * rewrite compileF_length; eauto.
         rewrite (take_eta k (getAnn ⊝ als)). rewrite countTrue_app.
@@ -161,16 +178,27 @@ Proof.
       * exploit IHIC2 as IH; eauto.
         rewrite zip_app in IH; eauto with len.
         erewrite <- getAnn_take_eq in IH; eauto.
-  - eapply IsCalledLet.
-    exploit IHIC; eauto; try reflexivity.
-    rewrite compileF_length; eauto.
-    rewrite zip_app in H; eauto with len.
-    rewrite take_app_ge in H; eauto 20 with len.
-    rewrite zip_length2 in H; eauto with len.
-    rewrite map_length in H.
-    orewrite (❬F❭ + n - ❬als❭ = n) in H. simpl.
-    rewrite map_app in H. rewrite countTrue_app in H.
-    rewrite <- getAnn_eq in H; eauto.
+  - cases.
+    + rewrite <- zip_app; eauto with len. exploit IHIC; eauto. reflexivity.
+      rewrite zip_app in H; eauto with len.
+      rewrite take_app_ge in H; eauto 20 with len.
+      rewrite zip_length2 in H; eauto with len.
+      rewrite map_length in H.
+      orewrite (❬F❭ + n - ❬als❭ = n) in H. simpl.
+      rewrite map_app in H. rewrite countTrue_app in H.
+      rewrite <- getAnn_eq in H; eauto.
+      erewrite <- compileF_length in H; eauto.
+      erewrite <- Heq in H. eauto.
+    + rewrite Heq. eapply IsCalledLet.
+      exploit IHIC; eauto; try reflexivity.
+      rewrite compileF_length; eauto.
+      rewrite zip_app in H; eauto with len.
+      rewrite take_app_ge in H; eauto 20 with len.
+      rewrite zip_length2 in H; eauto with len.
+      rewrite map_length in H.
+      orewrite (❬F❭ + n - ❬als❭ = n) in H. simpl.
+      rewrite map_app in H. rewrite countTrue_app in H.
+      rewrite <- getAnn_eq in H; eauto.
 Qed.
 
 Lemma DVE_noUnreachableCode ZL RL s lv
@@ -178,7 +206,9 @@ Lemma DVE_noUnreachableCode ZL RL s lv
     -> noUnreachableCode (compile (pair ⊜ RL ZL) s lv).
 Proof.
   intros Live. induction Live; simpl; repeat cases; eauto using noUnreachableCode.
-  - subst. econstructor; eauto using noUnreachableCode.
+  - rewrite <- zip_app; eauto with len.
+  - rewrite Heq; clear Heq.
+    econstructor; eauto using noUnreachableCode.
     + intros. destruct Zs as [Z' s'].
       edestruct compileF_get_inv as [Zs' [a [n' ?]]]; eauto; dcr; subst; simpl.
       rewrite <- zip_app; eauto with len.
@@ -191,178 +221,6 @@ Proof.
       exploit DVE_isCalled as IH; eauto.
       rewrite zip_app in IH; eauto with len.
       erewrite <- getAnn_take_eq in IH; eauto.
-Qed.
-
-Require Import paco2.
-
-(* A proof relation is parameterized by analysis information A *)
-Class ProofRelationI (A:Type) := {
-    (* Relates parameter lists according to analysis information *)
-    ParamRelI : A -> list var -> list var -> Prop;
-    (* Relates argument lists according to analysis information
-       and closure environments *)
-    ArgRelI : onv val -> onv val -> A-> list val -> list val -> Prop;
-    (* Relates blocks according to analysis information *)
-    BlockRelI : A -> I.block -> I.block -> Prop;
-    (* Relates environments according to analysis information *)
-    IndexRelI : 〔A〕 -> nat -> nat -> Prop;
-    Image : 〔A〕 -> nat;
-    ArgLengthMatchI : forall E E' a Z Z' VL VL',
-        ParamRelI a Z Z' -> ArgRelI E E' a VL VL' -> length Z = length VL /\ length Z' = length VL';
-    IndexRelDrop : forall AL' AL n n', IndexRelI (AL' ++ AL) n n' ->
-                                  n >= length AL'
-                                  -> IndexRelI AL (n - length AL') (n' - Image AL')
-(*    IndexRelApp : forall AL AL' n n', IndexRelI AL n n' -> IndexRelI (AL' ++ AL) (❬AL'❭ + n) n' *)
-}.
-
-Definition indexwise_r (r:rel2 I.state (fun _ => I.state)) A (PR:ProofRelationI A) AL' F F' AL L L' :=
-  forall n n' Z s Z' s' a,
-    IndexRelI (AL' ++ AL) n n'
-    -> get F n (Z,s)
-    -> get F' n' (Z',s')
-    -> get AL' n a
-    -> forall E E' VL VL',
-        ArgRelI E E' a VL VL'
-        -> r (mapi I.mkBlock F ++ L, E[Z <-- List.map Some VL], s)
-            (mapi I.mkBlock F' ++ L', E'[Z' <-- List.map Some VL'], s').
-
-Lemma indexwise_r_mon (r r':rel2 I.state (fun _ => I.state)) A (PR:ProofRelationI A) AL' F F' AL L L'
-  : indexwise_r r PR AL' F F' AL L L'
-    -> (forall x y, r x y -> r' x y)
-    -> indexwise_r r' PR AL' F F' AL L L'.
-Proof.
-  intros Idx LE; hnf; intros; eauto.
-Qed.
-
-Definition renILabenv r
-           {A} (PR:ProofRelationI A) (AL:list A) L L' :=
-  (length AL = length L /\ sawtooth L' /\ sawtooth L) /\
-  forall f f' a Z s n Z' s' n',
-    IndexRelI AL f f'
-    -> get AL f a
-    -> get L f (I.blockI Z s n)
-    -> get L' f' (I.blockI Z' s' n')
-    -> (ParamRelI a Z Z' /\ BlockRelI a (I.blockI Z s n) (I.blockI Z' s' n'))
-      /\ (forall E E' Yv Y'v Y Y',
-            ArgRelI E E' a Yv Y'v
-            -> omap (exp_eval E) Y = Some Yv
-            -> omap (exp_eval E') Y' = Some Y'v
-            -> sim'r r (drop (f  - n) L, E, stmtApp (LabI n) Y)
-                    (drop (f'  - n') L', E', stmtApp (LabI n') Y')).
-
-Lemma renILabenv_mon (r r':rel2 I.state (fun _ => I.state)) A (PR:ProofRelationI A) AL L L'
-  : renILabenv r PR AL L L'
-    -> (forall x y, r x y -> r' x y)
-    -> renILabenv r' PR AL L L'.
-Proof.
-  intros [[? ?] SIM] LE; hnf; intros; split; eauto.
-  intros. edestruct SIM as [[? ?] SIM']; eauto.
-  split; eauto. intros.
-  eapply paco2_mon. eapply SIM; eauto. eauto.
-Qed.
-
-Definition indexwise_proofrel A (PR:ProofRelationI A) (F F':〔params * stmt〕) AL' AL :=
-  forall n n' Z s Z' s' a,
-    IndexRelI (AL' ++ AL) n n'
-    -> get F n (Z,s)
-    -> get F' n' (Z',s')
-    -> get AL' n a
-    -> ParamRelI a Z Z' /\ BlockRelI a (I.blockI Z s n) (I.blockI Z' s' n').
-
-Lemma renILabenv_extension' r A (PR:ProofRelationI A) (AL AL':list A) F F' L L'
-      (LEN1:length AL' = length F)
-  : indexwise_r (sim'r r \2/ r) PR AL' F F' AL L L'
-    -> indexwise_proofrel PR F F' AL' AL
-    -> (forall n n', IndexRelI (AL' ++ AL) n n' -> n < length F -> n' < length F')
-    -> (forall n n', IndexRelI (AL' ++ AL) n n' -> n >= length F -> n' >= length F')
-    -> Image AL' = length F'
-    -> renILabenv r PR AL L L'
-    -> renILabenv r PR (AL' ++ AL) (mapi I.mkBlock F ++ L) (mapi I.mkBlock F' ++ L').
-Proof.
-  intros ISIM IP Ilt Ige Img SIML.
-  hnf. split.
-  destruct SIML; dcr; split; eauto with len. split; eauto.
-  econstructor; eauto. eapply tooth_I_mkBlocks.
-  econstructor; eauto. eapply tooth_I_mkBlocks.
-  intros ? ? ? ? ? ? ? ? ? RN GetAL GetFL GetL'.
-  assert (❬AL'❭ = ❬mapi I.mkBlock F❭) by eauto with len.
-  eapply get_app_cases in GetAL. destruct GetAL as [GetAL'|GetAL].
-  - eapply get_app_lt_1 in GetFL; [| rewrite <- H; eauto using get_range].
-    inv_get. destruct x as [Z s]. simpl in *. clear EQ.
-    orewrite (n - n = 0). simpl.
-    exploit Ilt; eauto using get_range.
-    eapply get_app_lt_1 in GetL'; [| rewrite mapi_length; eauto with len ].
-    inv_get. destruct x as [Z' s']; simpl in *; clear EQ.
-    split; eauto.
-    intros.
-    exploit (ArgLengthMatchI); eauto; dcr. eapply IP; eauto.
-    pone_step; eauto using get_app, get_mapi; eauto using get_app, mapi_get_1; simpl; eauto with len.
-    orewrite (n' - n' = 0); simpl.
-    eapply get_app. eapply mapi_get_1; eauto.
-    simpl. eauto with len.
-    orewrite (n - n = 0); simpl.
-    orewrite (n' - n' = 0); simpl.
-    eapply ISIM; eauto.
-  - destruct SIML; dcr.
-    eapply get_app_right_ge in GetFL; [ | rewrite <- H; eauto].
-    exploit Ige; eauto; try congruence.
-    eapply get_app_right_ge in GetL'; [ | eauto with len; rewrite mapi_length; eauto].
-    rewrite mapi_length in *.
-    eapply IndexRelDrop in RN; eauto.
-    edestruct H1 as [[? ?] SIM]; eauto. rewrite H; eauto. rewrite Img; eauto.
-    split; eauto.
-    intros.
-    assert (f - n >= ❬mapi I.mkBlock F❭). {
-      exploit (sawtooth_smaller H7 GetFL).
-      rewrite <- H in *. rewrite mapi_length. simpl in *. omega.
-    }
-    assert (f' - n' >= ❬mapi I.mkBlock F'❭). {
-      exploit (sawtooth_smaller H6 GetL').
-      rewrite mapi_length in *.
-      simpl in *. omega.
-    }
-    rewrite (drop_app_gen _ (mapi I.mkBlock F)); eauto.
-    rewrite (drop_app_gen _ (mapi I.mkBlock F')); eauto.
-    repeat rewrite mapi_length. rewrite H in SIM. rewrite Img in SIM.
-    orewrite (f - n - ❬F❭ = f - ❬F❭ - n).
-    orewrite (f' - n' - ❬F'❭ = f' - ❬F'❭ - n').
-    eapply paco2_mon. eapply SIM; eauto. eauto.
-Qed.
-
-Lemma fix_compatible_I A (PR:ProofRelationI A) AL F F' L L' AL'
-(LEN2:length AL' = length F)
-  : (forall r, renILabenv r PR (AL' ++ AL) (mapi I.mkBlock F ++ L) (mapi I.mkBlock F' ++ L')
-            -> indexwise_r (sim'r r) PR AL' F F' AL L L')
-    -> indexwise_proofrel PR F F' AL' AL
-    -> (forall n n', IndexRelI (AL' ++ AL) n n' -> n < length F -> n' < length F')
-    -> (forall n n', IndexRelI (AL' ++ AL) n n' -> n >= length F -> n' >= length F')
-    -> Image AL' = length F'
-    -> forall r, renILabenv r PR AL L L'
-           -> indexwise_r (sim'r r) PR AL' F F' AL L L'.
-Proof.
-  intros ISIM IP Ilt Ige Img r SIML; pcofix CIH.
-  eapply ISIM; eauto.
-  hnf. split.
-  destruct SIML; dcr; split; eauto with len. split.
-  econstructor; eauto. eapply tooth_I_mkBlocks.
-  econstructor; eauto. eapply tooth_I_mkBlocks.
-  eapply renILabenv_extension'; eauto using renILabenv_mon, indexwise_r_mon.
-Qed.
-
-Lemma renILabenv_extension A (PR:ProofRelationI A) (AL AL':list A) F F' L L'
-      (LEN1:length AL' = length F)
-  : (forall r, renILabenv r PR (AL' ++ AL) (mapi I.mkBlock F ++ L) (mapi I.mkBlock F' ++ L')
-          -> indexwise_r (sim'r r) PR AL' F F' AL L L')
-    -> indexwise_proofrel PR F F' AL' AL
-    -> (forall n n', IndexRelI (AL' ++ AL) n n' -> n < length F -> n' < length F')
-    -> (forall n n', IndexRelI (AL' ++ AL) n n' -> n >= length F -> n' >= length F')
-    -> Image AL' = length F'
-    -> forall r, renILabenv r PR AL L L'
-           -> renILabenv r PR (AL' ++ AL) (mapi I.mkBlock F ++ L) (mapi I.mkBlock F' ++ L').
-Proof.
-  intros. eapply renILabenv_extension'; eauto.
-  eapply indexwise_r_mon.
-  eapply fix_compatible_I; eauto. eauto.
 Qed.
 
 Module I.
@@ -426,13 +284,13 @@ Qed.
 
 Lemma sim_I ZL RL r L L' V s a
 : unreachable_code ZL RL s a
--> renILabenv r SR (pair ⊜ RL ZL) L L'
+-> simILabenv Bisim r SR (pair ⊜ RL ZL) L L'
 -> (forall (f:nat) Z,
       get (pair ⊜ RL ZL) f (true, Z)
       -> exists (b b' : I.block),
         get L f b /\
         get L' (countTrue (fst ⊝ (take f (pair ⊜ RL ZL)))) b')
--> sim'r r (L,V, s) (L',V, compile (pair ⊜ RL ZL) s a).
+-> sim'r r Bisim (L,V, s) (L',V, compile (pair ⊜ RL ZL) s a).
 Proof.
   unfold sim'r. revert_except s.
   sind s; destruct s; simpl; intros; invt unreachable_code; simpl in * |- *.
@@ -462,84 +320,124 @@ Proof.
       econstructor 3; eauto.
       econstructor 3; eauto.
       left; eapply (IH s2); eauto using agree_on_incl.
-      pfold. econstructor 3; try eapply star2_refl; eauto.
-      stuck.
+      pfold. econstructor 4; try eapply star2_refl; eauto.
+      stuck. stuck.
   - edestruct H1 as [? [? [GetL GetL']]]; eauto using zip_get.
     remember (omap (exp_eval V) Y). symmetry in Heqo.
     destruct o.
     + destruct x as [Z1 s1 n1], x0 as [Z2 s2 n2].
-      edestruct H0 as [[? ?] SIM]; eauto.
+      edestruct H0 as [[? ?] SIM]; eauto; dcr.
       edestruct SIM as [[? ?] SIM']; eauto using zip_get.
       hnf; simpl. split; eauto using zip_get.
-      hnf in H5. simpl in *; dcr. subst Z1. subst Z2.
-      eapply (@sim_Y_left I.state _ I.state _).
-      eapply (@sim_Y_right I.state _ I.state _).
+      instantiate (1:=LabI (countTrue (fst ⊝ take (labN l) (pair ⊜ RL ZL)))).
+      reflexivity. simpl. eauto.
       eapply SIM'; eauto using zip_get.
-      hnf; simpl. split; eauto using zip_get.
-      hnf; intros; simpl; eauto with len.
-      Focus 4. econstructor; eauto with len.
-      Focus 2. econstructor; eauto. simpl.
-      * simpl.
-        eapply (stepGoto' _ _ GetL'); eauto; simpl.
-      * simpl.
-        eapply (stepGoto' _ _ GetL); eauto.
-    + pfold; econstructor 3; try eapply star2_refl; eauto; stuck2.
-
+      hnf; simpl. split; eauto using zip_get with len.
+    + pfold; econstructor 4; try eapply star2_refl; eauto; stuck2.
   - pno_step.
   - remember (omap (exp_eval V) Y). symmetry in Heqo.
     destruct o.
     + pextern_step; eauto using agree_on_update_same, agree_on_incl; try congruence.
     + pno_step.
-  - pone_step. left. rewrite <- zip_app; eauto with len.
-    eapply IH; eauto.
-    + rewrite zip_app; eauto with len.
-      eapply renILabenv_extension; eauto. eauto with len.
-      * intros. hnf; intros.
-        hnf in H3. dcr. hnf in H11; dcr; subst.
-        rewrite get_app_lt in H14; eauto using get_range.
-        inv_get.
-        exploit (compileF_get ((pair ⊜ (getAnn ⊝ als) (fst ⊝ s) ++ pair ⊜ RL ZL) )); eauto.
-        erewrite <- getAnn_take_eq in H7; eauto.
-        simpl in *. get_functional.
-        rewrite <- zip_app; eauto with len.
-        eapply IH; eauto. exploit H8; eauto.
-        rewrite zip_app; eauto with len.
-        intros.
-        eapply inv_extend; eauto with len.
-      * hnf; intros.
-        hnf in H2. dcr; subst.
-        rewrite get_app_lt in H12; eauto with len.
-        inv_get. simpl; unfold ParamRel; simpl.
-        exploit (compileF_get ((pair ⊜ (getAnn ⊝ als) (fst ⊝ s) ++ pair ⊜ RL ZL) )); eauto.
-        erewrite <- getAnn_take_eq in H6; eauto.
-        get_functional. eauto.
-      * intros. rewrite compileF_length; eauto.
-        hnf in H2; dcr; subst.
-        rewrite get_app_lt in H9;
-          [| rewrite zip_length2; eauto with len; rewrite map_length; omega].
-        inv_get.
-        erewrite <- getAnn_take_eq; eauto.
-        rewrite map_take.
-        erewrite (take_eta n (getAnn ⊝ als)) at 2.
-        rewrite countTrue_app.
-        erewrite <- get_eq_drop; eauto using map_get_1.
-        rewrite EQ1. simpl; omega.
-      * intros. rewrite compileF_length; eauto.
-        hnf in H2; dcr; subst.
+  - cases.
+    + eapply sim'_expansion_closed;
+        [| eapply star2_silent; [ econstructor; eauto | eapply star2_refl ]
+         | eapply star2_refl ].
+      rewrite <- zip_app; eauto with len.
+      eapply IH; eauto.
+      * rewrite zip_app; eauto with len.
+        eapply simILabenv_extension with (F':=nil); eauto. eauto with len.
+        intros; isabsurd. isabsurd.
+        simpl; intros; dcr; subst. exfalso.
+        rewrite get_app_lt in H9; eauto with len. inv_get.
+        assert (length (compileF compile (pair ⊜ (getAnn ⊝ als) (fst ⊝ s) ++ pair ⊜ RL ZL) s als)
+                <> 0). {
+          rewrite compileF_length; eauto.
+          eapply countTrue_exists. rewrite <- EQ1; eauto using map_get_1.
+        }
+        eapply H6. rewrite <- Heq. eauto.
+        simpl; intros; dcr; subst.
+        rewrite get_app_ge in H9; eauto with len. inv_get.
         rewrite map_take. rewrite map_app.
         rewrite map_zip.
         rewrite zip_map_fst; eauto with len.
         rewrite take_app_ge. rewrite countTrue_app. omega.
         rewrite map_length. omega.
-      * simpl. rewrite compileF_length; eauto.
-        rewrite map_zip.
-        rewrite zip_map_fst; eauto with len.
-    + rewrite zip_app; eauto with len. intros; eapply inv_extend; eauto.
+        rewrite zip_length2; eauto with len.
+        rewrite map_length. omega.
+        simpl. rewrite <- getAnn_eq; eauto. erewrite <- compileF_length; eauto.
+        erewrite <- Heq. eauto.
+      * intros. rewrite zip_app in H2; eauto with len.
+        eapply get_app_cases in H2. destruct H2.
+        exfalso. inv_get.
+        assert (length (compileF compile (pair ⊜ (getAnn ⊝ als) (fst ⊝ s) ++ pair ⊜ RL ZL) s als)
+                <> 0). {
+          rewrite compileF_length; eauto.
+          eapply countTrue_exists. rewrite <- EQ1; eauto using map_get_1.
+        }
+        eapply H6. rewrite <- Heq. eauto.
+        dcr. exploit H1; eauto. destruct H2 as [? [? ?]]; dcr.
+        do 2 eexists. split.
+        eapply get_app_right; eauto. rewrite mapi_length, zip_length2; eauto with len.
+        rewrite map_length. rewrite zip_length2 in H6; eauto with len.
+        rewrite map_length in H6. omega.
+        rewrite zip_app; eauto with len.
+        rewrite take_app_ge; eauto. rewrite map_app.
+        rewrite <- getAnn_eq; eauto. rewrite countTrue_app.
+        erewrite <- compileF_length; eauto. erewrite <- Heq. eauto.
+    + rewrite Heq; clear Heq.
+      pone_step. left. rewrite <- zip_app; eauto with len.
+      eapply IH; eauto.
+      {
+        + rewrite zip_app; eauto with len.
+          eapply simILabenv_extension; eauto. eauto with len.
+          * intros. hnf; intros.
+            hnf in H3. dcr. hnf in H11; dcr; subst.
+            rewrite get_app_lt in H14; eauto using get_range.
+            inv_get.
+            exploit (compileF_get ((pair ⊜ (getAnn ⊝ als) (fst ⊝ s) ++ pair ⊜ RL ZL) )); eauto.
+            erewrite <- getAnn_take_eq in H7; eauto.
+            simpl in *. get_functional.
+            rewrite <- zip_app; eauto with len.
+            eapply IH; eauto. exploit H8; eauto.
+            rewrite zip_app; eauto with len.
+            intros.
+            eapply inv_extend; eauto with len.
+          * hnf; intros.
+            hnf in H2. dcr; subst.
+            rewrite get_app_lt in H12; eauto with len.
+            inv_get. simpl; unfold ParamRel; simpl.
+            exploit (compileF_get ((pair ⊜ (getAnn ⊝ als) (fst ⊝ s) ++ pair ⊜ RL ZL) )); eauto.
+            erewrite <- getAnn_take_eq in H6; eauto.
+            get_functional. eauto.
+          * intros. rewrite compileF_length; eauto.
+            hnf in H2; dcr; subst.
+            rewrite get_app_lt in H9;
+              [| rewrite zip_length2; eauto with len; rewrite map_length; omega].
+            inv_get.
+            erewrite <- getAnn_take_eq; eauto.
+            rewrite map_take.
+            erewrite (take_eta n (getAnn ⊝ als)) at 2.
+            rewrite countTrue_app.
+            erewrite <- get_eq_drop; eauto using map_get_1.
+            rewrite EQ1. simpl; omega.
+          * intros. rewrite compileF_length; eauto.
+            hnf in H2; dcr; subst.
+            rewrite map_take. rewrite map_app.
+            rewrite map_zip.
+            rewrite zip_map_fst; eauto with len.
+            rewrite take_app_ge. rewrite countTrue_app. omega.
+            rewrite map_length. omega.
+          * simpl. rewrite compileF_length; eauto.
+            rewrite map_zip.
+            rewrite zip_map_fst; eauto with len.
+      }
+      rewrite zip_app; eauto with len. intros; eapply inv_extend; eauto.
 Qed.
 
 Lemma sim_DVE V s a
 : unreachable_code nil nil s  a
--> @sim I.state _ I.state _ (nil,V, s) (nil,V, compile nil s a).
+-> @sim I.state _ I.state _ Bisim (nil,V, s) (nil,V, compile nil s a).
 Proof.
   intros. eapply sim'_sim.
   eapply (@sim_I nil nil); eauto; isabsurd.
@@ -548,233 +446,23 @@ Qed.
 
 End I.
 
-
-Definition ArgRel (V V:onv val) (G:option (set var * params)) (VL VL': list val) : Prop :=
-  match G with
-  | Some G => VL' = (filter_by (fun x => B[x ∈ (fst G)]) (snd G) VL) /\ length (snd G) = length VL
-  | None => VL' = VL
-  end.
-
-Definition ParamRel (G:(؟(set var * params))) (Z Z' : list var) : Prop :=
-  match G with
-  | Some G => Z' = (List.filter (fun x => B[x ∈ (fst G)]) Z) /\ snd G = Z
-  | None => True
-  end.
-
-Instance SR : ProofRelationI (؟(set var * params)) :=
-  {
-    ParamRelI := ParamRel;
-    ArgRelI := ArgRel;
-    BlockRelI := fun lvZ b b' => True;
-    IndexRelI D n n' := True
-  }.
-Proof.
-intros. hnf in H, H0. destruct a; dcr. subst.
-erewrite filter_filter_by_length; eauto.
-Admitted.
-
-
-Fixpoint compile_live (s:stmt) (a:ann (set var)) (G:set var) : ann (set var) :=
+Fixpoint compile_live (s:stmt) (a:ann (set var)) : ann (set var) :=
   match s, a with
     | stmtLet x e s, ann1 lv an as a =>
-      if [x ∈ getAnn an] then ann1 (G ∪ lv) (compile_live s an {x})
-                         else compile_live s an G
+      ann1 lv (compile_live s an)
     | stmtIf e s t, ann2 lv ans ant =>
       if [exp2bool e = Some true] then
-        compile_live s ans G
+        compile_live s ans
       else if [exp2bool e = Some false ] then
-        compile_live t ant G
+        compile_live t ant
       else
-        ann2 (G ∪ lv) (compile_live s ans ∅) (compile_live t ant ∅)
-    | stmtApp f Y, ann0 lv => ann0 (G ∪ lv)
-    | stmtReturn x, ann0 lv => ann0 (G ∪ lv)
+        ann2 lv (compile_live s ans) (compile_live t ant)
+    | stmtApp f Y, ann0 lv => ann0 lv
+    | stmtReturn x, ann0 lv => ann0 lv
     | stmtExtern x f Y s, ann1 lv an as a =>
-      ann1 (G ∪ lv) (compile_live s an {x})
+      ann1 lv (compile_live s an)
     | stmtFun F t, annF lv ans ant =>
-      let ans' := zip (fun Zs a => let a' := compile_live (snd Zs) a ∅ in
-                               setTopAnn a' (getAnn a' ∪ of_list (List.filter (fun x => B[x ∈ getAnn a]) (fst Zs)))) F ans in
-      annF (G ∪ lv) ans' (compile_live t ant ∅)
+      let ans' := zip (fun Zs a => compile_live (snd Zs) a) F ans in
+      annF lv ans' (compile_live t ant)
     | _, a => a
   end.
-
-
-Lemma compile_live_incl G i LV s lv
-  : true_live_sound i LV s lv
-    -> getAnn (compile_live s lv G) ⊆ G ∪ getAnn lv.
-Proof.
-  intros. general induction H; simpl; eauto.
-  - cases; simpl; try reflexivity.
-    rewrite IHtrue_live_sound. rewrite <- H1. cset_tac; intuition.
-  - repeat cases; simpl; try reflexivity.
-    + etransitivity; eauto. rewrite <- H2. eauto. congruence.
-    + etransitivity; eauto.  rewrite <- H3; eauto.
-Qed.
-
-Lemma compile_live_incl_empty i LV s lv
-  : true_live_sound i LV s lv
-    -> getAnn (compile_live s lv ∅) ⊆ getAnn lv.
-Proof.
-  intros.
-  eapply compile_live_incl in H.
-  rewrite H. cset_tac; intuition.
-Qed.
-
-Lemma incl_compile_live G i LV s lv
-  : true_live_sound i LV s lv
-    -> G ⊆ getAnn (compile_live s lv G).
-Proof.
-  intros. general induction H; simpl; eauto.
-  - cases; simpl; try reflexivity. cset_tac; intuition.
-    rewrite <- IHtrue_live_sound. cset_tac; intuition.
-  - repeat cases; simpl; try reflexivity; eauto.
-Qed.
-
-Definition compile_LV (LV:list (set var *params)) :=
-  List.map (fun lvZ => let Z' := List.filter (fun x => B[x ∈ fst lvZ]) (snd lvZ) in
-                      (fst lvZ, Z')) LV.
-
-Lemma dve_live i LV s lv G
-  : true_live_sound i LV s lv
-    -> live_sound i (compile_LV LV) (compile LV s lv) (compile_live s lv G).
-Proof.
-  intros. general induction H; simpl; eauto using live_sound, compile_live_incl.
-  - cases; eauto. econstructor; eauto.
-    + eapply live_exp_sound_incl; eauto. eauto.
-    + rewrite compile_live_incl; eauto.
-      rewrite <- H1. cset_tac; intuition.
-    + eapply incl_compile_live; eauto.
-  - repeat cases; eauto.
-    + econstructor; eauto; try rewrite compile_live_incl; eauto.
-      eapply live_exp_sound_incl. eapply incl_right.
-      eapply H1. case_eq (exp2bool e); intros; try destruct b; congruence.
-      cset_tac; intuition.
-      cset_tac; intuition.
-  - econstructor.
-    + eapply (map_get_1 (fun lvZ => let Z' := List.filter (fun x => B[x ∈ fst lvZ]) (snd lvZ) in
-                                   (fst lvZ, Z')) H); eauto.
-    + simpl. destruct i; simpl in * |- *; eauto.
-      rewrite <- H0. rewrite minus_inter_empty. eapply incl_right.
-      cset_tac; intuition. eapply filter_incl2; eauto.
-      eapply filter_in; eauto. intuition. hnf. cases; eauto.
-      rewrite <- H0. rewrite minus_inter_empty. eapply incl_right.
-      cset_tac; intuition. eapply filter_incl2; eauto.
-      eapply filter_in; eauto. intuition. hnf. cases; eauto.
-    + simpl. eapply get_nth in H. erewrite H. simpl.
-      erewrite filter_filter_by_length. reflexivity. congruence.
-    + intros. eapply get_nth in H. erewrite H in H3. simpl in *.
-      edestruct filter_by_get as [? [? [? []]]]; eauto; dcr.
-      eapply live_exp_sound_incl. eapply incl_right.
-      eapply argsLive_live_exp_sound; eauto. simpl in *.
-      decide (x0 ∈ blv); intuition.
-  - econstructor; eauto.
-    eapply live_exp_sound_incl; eauto using incl_right.
-  - econstructor; eauto.
-    + intros; eapply live_exp_sound_incl; eauto using incl_right.
-    + rewrite compile_live_incl; eauto. rewrite <- H1. cset_tac; intuition.
-    + eapply incl_compile_live; eauto.
-  - econstructor; simpl in *; eauto with len.
-    + eapply live_sound_monotone.
-      eapply IHtrue_live_sound.
-      unfold compile_LV. rewrite map_app. eapply PIR2_app; eauto.
-      eapply PIR2_get; eauto 30 with len.
-      intros; inv_get. simpl. rewrite getAnn_setTopAnn.
-      rewrite compile_live_incl_empty; eauto. rewrite of_list_filter.
-      split; cset_tac.
-    + intros; inv_get.
-      eapply live_sound_monotone.
-      eapply live_sound_monotone2; eauto. eapply H2; eauto.
-      unfold compile_LV. rewrite map_app. eapply PIR2_app; eauto.
-      eapply PIR2_get; eauto 30 with len.
-      intros; inv_get. simpl. rewrite getAnn_setTopAnn.
-      rewrite compile_live_incl_empty; eauto. rewrite of_list_filter.
-      split; cset_tac.
-    + intros; inv_get.
-      repeat rewrite getAnn_setTopAnn; simpl.
-      split; eauto. cases; eauto.
-      exploit H3; eauto.
-      rewrite compile_live_incl_empty; eauto. rewrite <- H5.
-      rewrite of_list_filter.
-      clear_all; cset_tac.
-    + rewrite compile_live_incl; eauto with cset.
-Qed.
-
-Lemma sim_DVE' r L L' V V' s LV lv
-: agree_on eq (getAnn lv) V V'
--> true_live_sound Functional LV s lv
--> simL' sim_progeq r SR LV L L'
--> sim'r r (L,V, s) (L',V', compile LV s lv).
-Proof.
-  unfold simL', sim'r. revert_except s.
-  sind s; destruct s; simpl; intros; invt true_live_sound; simpl in * |- *.
-  - case_eq (exp_eval V e); intros. cases.
-    + pone_step.
-      instantiate (1:=v). erewrite exp_eval_live; eauto. eapply agree_on_sym; eauto.
-      left. eapply (IH s); eauto. eapply agree_on_update_same; eauto with cset.
-    + eapply sim'_expansion_closed;
-      [ | eapply S_star2 with (y:=EvtTau);
-          [ econstructor; eauto | eapply star2_refl ]
-        | eapply star2_refl].
-      eapply (IH s); eauto. eapply agree_on_update_dead; eauto with cset.
-    + pfold. econstructor 3; [| eapply star2_refl|]; eauto. stuck.
-  - repeat cases.
-    + edestruct (exp2bool_val2bool V); eauto; dcr.
-      eapply sim'_expansion_closed.
-      eapply (IH s1); eauto. eapply agree_on_incl; eauto.
-      eapply H10; congruence.
-      eapply S_star2 with (y:=EvtTau) (yl:=nil).
-      econstructor; eauto. eapply star2_refl.
-      eapply star2_refl.
-    + edestruct (exp2bool_val2bool V); eauto; dcr.
-      eapply sim'_expansion_closed.
-      eapply (IH s2); eauto. eapply agree_on_incl; eauto.
-      eapply S_star2 with (y:=EvtTau) (yl:=nil).
-      econstructor 3; eauto. eapply star2_refl.
-      eapply star2_refl.
-    + remember (exp_eval V e). symmetry in Heqo.
-      exploit exp_eval_live_agree; eauto.
-      eapply H8. case_eq (exp2bool e); intros; try destruct b; congruence.
-      destruct o. case_eq (val2bool v); intros.
-      pone_step. left. eapply IH; eauto with cset.
-      pone_step. left; eapply (IH s2); eauto with cset.
-      pno_step.
-  - destruct (get_dec L (counted l)) as [[[bE bZ bs]]|].
-    + remember (omap (exp_eval V) Y). symmetry in Heqo.
-      rewrite (get_nth (∅, nil) H4); simpl.
-      destruct o.
-      * exploit omap_filter_by; eauto.
-        unfold simL' in H1. inRel_invs. simpl in *.
-        hnf in H17; dcr; subst; simpl in *.
-        eapply sim_drop_shift; eauto.
-        eapply (inRel_sawtooth H1). eapply (inRel_sawtooth H1). eapply H19. eauto.
-        eapply omap_exp_eval_live_agree; eauto.
-        eapply argsLive_liveSound; eauto.
-        hnf; split; eauto. simpl. exploit omap_length; try eapply Heqo; eauto.
-        congruence.
-      * pfold; econstructor 3; try eapply star2_refl; eauto; stuck2.
-    + pfold; econstructor 3; try eapply star2_refl; eauto; stuck2.
-  - pno_step; simpl. erewrite <- exp_eval_live_agree; eauto; symmetry; eauto.
-  - remember (omap (exp_eval V) Y). symmetry in Heqo.
-    exploit omap_exp_eval_live_agree; eauto.
-    destruct o.
-    + pextern_step; eauto using agree_on_update_same, agree_on_incl; try congruence.
-    + pno_step.
-  - pone_step. left. eapply IH; eauto with cset.
-    + eapply simL_mon; eauto. eapply simL_extension'; eauto with len.
-      * intros. inv_get; simpl. split. hnf; intros; simpl.
-        unfold ParamRel, ArgRel. intuition.
-        eapply (IH s1); eauto. subst.
-        eapply agree_on_update_filter'; eauto.
-        eapply agree_on_incl; eauto. simpl.
-        exploit H8; eauto.
-        exploit H6; eauto.
-        unfold ParamRel. intuition.
-Qed.
-
-Lemma sim_DVE V V' s lv
-: agree_on eq (getAnn lv) V V'
--> true_live_sound Functional nil s lv
--> @sim F.state _ F.state _ (nil,V, s) (nil,V', compile nil s lv).
-Proof.
-  intros. eapply sim'_sim.
-  eapply sim_DVE'; eauto. hnf. econstructor.
-Qed.
